models/simlin/TPSimulation.v
@@ -8,6 +8,7 @@ Require Import LinCCAL.
 Require Import LTS.
 Require Import Lang.
 Require Import Semantics.
+Require Import TPSimulationSet.
 
 (* threadpool simulation *)
 Module TPSimulation.
@@ -75,4 +76,112 @@ Module TPSimulation.
     li_correct : cal li_impl (li_init L) (li_init L');
   }.
   Arguments layer_implementation : clear implicits.
+
+  Definition to_set_layer_interface (L : layer_interface) :
+    TPSimulationSet.TPSimulation.layer_interface :=
+  {|
+    TPSimulationSet.TPSimulation.li_sig := li_sig L;
+    TPSimulationSet.TPSimulation.li_lts := li_lts L;
+    TPSimulationSet.TPSimulation.li_init := li_init L;
+  |}.
+
+  Section SingletonLift.
+    Context {E : Op.t}.
+    Context {F : Op.t}.
+    Context {VE : @LTS E}.
+    Context {VF : @LTS F}.
+    Context (M : ModuleImpl E F).
+
+    Lemma ac_singleton_subset_steps
+        (Δ : Semantics.AbstractConfig VF) (ρ ρ' : State VF)
+        (π π' : tmap (@LinState F))
+        (Hequiv : ac_equiv Δ (ac_singleton ρ π))
+        (Hsteps : poss_steps (PossOk ρ π) (PossOk ρ' π')) :
+      (ac_singleton ρ' π' ⊆ ac_steps Δ)%AbstractConfig.
+    Proof.
+      intros ρ0 π0 Hsingle.
+      inversion Hsingle; subst.
+      econstructor; eauto.
+      apply Hequiv. constructor.
+    Qed.
+
+    Theorem TPSimulation_singleton_lift σ c ρ π :
+      TPSimulation M σ c ρ π ->
+      forall (Δ : Semantics.AbstractConfig VF),
+        ac_equiv Δ (ac_singleton ρ π) ->
+        @TPSimulationSet.TPSimulation.TPSimulation E F VE VF M σ c Δ.
+    Proof.
+      revert σ c ρ π.
+      cofix CIH.
+      intros σ c ρ π HTPSim Δ Hequiv.
+      inversion HTPSim; subst.
+      - eapply TPSimulationSet.TPSimulation.TPSim_Error with (ρ := ρ) (π := π);
+          eauto.
+        apply Hequiv. constructor.
+      - apply TPSimulationSet.TPSimulation.TPSim_Continue.
+        + intros t f c' Hstep.
+          eapply CIH; eauto.
+          intros ρ0 π0. split; intro H.
+          * inversion H; subst.
+            apply Hequiv in Hposs.
+            inversion Hposs; subst.
+            constructor.
+          * inversion H; subst.
+            constructor.
+            apply Hequiv. constructor.
+        + intros t f ret c' Hstep.
+          split.
+          * intros ρ0 π0 Hposs.
+            apply Hequiv in Hposs.
+            inversion Hposs; subst.
+            destruct (tpsim_retstep t f ret c' Hstep) as [? _].
+            auto.
+          * destruct (tpsim_retstep t f ret c' Hstep) as [_ Hsim].
+            eapply CIH; eauto.
+            intros ρ0 π0. split; intro H.
+            -- inversion H; subst.
+               apply Hequiv in Hposs.
+               inversion Hposs; subst.
+               constructor.
+            -- inversion H; subst.
+               constructor.
+               apply Hequiv. constructor.
+        + intros ev σ' c' Hstep.
+          destruct (tpsim_ustep ev σ' c' Hstep) as [ρ' [π' [Hsteps Hsim]]].
+          exists (ac_singleton ρ' π'). split.
+          * eapply ac_singleton_subset_steps; eauto.
+          * eapply CIH; eauto. reflexivity.
+        + destruct tpsim_linstep as [ρ' [π' [Hsteps Hsim]]].
+          exists (ac_singleton ρ' π'). split.
+          * eapply ac_singleton_subset_steps; eauto.
+          * eapply CIH; eauto. reflexivity.
+        + intros t c' Hstep.
+          eapply CIH; eauto.
+        + auto.
+    Qed.
+
+    Corollary TPSimulation_singleton σ c ρ π :
+      TPSimulation M σ c ρ π ->
+      @TPSimulationSet.TPSimulation.TPSimulation E F VE VF M σ c (ac_singleton ρ π).
+    Proof.
+      intros.
+      eapply TPSimulation_singleton_lift; eauto.
+      reflexivity.
+    Qed.
+  End SingletonLift.
+
+  Theorem layer_implementation_TPSimulationSet {L L' : layer_interface} :
+    layer_implementation L L' ->
+    TPSimulationSet.TPSimulation.layer_implementation
+      (to_set_layer_interface L) (to_set_layer_interface L').
+  Proof.
+    intros [M Hcorrect].
+    refine (@TPSimulationSet.TPSimulation.Build_layer_implementation
+              (to_set_layer_interface L) (to_set_layer_interface L') M _).
+    unfold TPSimulationSet.TPSimulation.cal,
+           TPSimulationSet.TPSimulation.ac_init,
+           cal in *.
+    apply TPSimulation_singleton.
+    exact Hcorrect.
+  Qed.
 End TPSimulation.
